txn-data-consistency/EP+_TCCv_update_kv_invs.thy
@@ -2,22 +2,63 @@ theory "EP+_TCCv_update_kv_invs"
   imports "EP+_TCCv_proof"
 begin
 
+lemma map_list_update:
+  "i < length (corder k) \<Longrightarrow> distinct (corder k) \<Longrightarrow>
+   (map f (corder k)) [i := x] = map (f ((corder k) ! i := x)) (corder k)"
+  by (smt (verit) fun_upd_apply length_list_update length_map nth_eq_iff_index_eq
+      nth_equalityI nth_list_update nth_map)
+
+lemma view_of_in_range:
+  assumes "i \<in> view_of corder ctx k"
+    and "ctx `` {k} \<subseteq> set (corder k)"
+    and "distinct (corder k)"
+  shows "i < length (corder k)"
+  using assms
+  apply (auto simp add: view_of_def Image_def)
+  by (smt (verit, best) distinct_Ex1 the1_equality)
+
+lemma finite_view_of:
+  "finite (view_of (commit_order s) ctx k)"
+  by (simp add: view_of_def)
+
+lemma view_of_non_emp:
+  assumes "T0_in_CO s k"
+    and "View_Init s cl"
+  shows "view_of (commit_order s) (cl_ctx (cls s cl) \<union> u) k \<noteq> {}"
+  using assms
+  by (auto simp add: view_of_def)
+
+lemma Max_view_of_in_range:
+  assumes "view_of corder ctx k \<noteq> {}"
+    and "finite (view_of corder ctx k)"
+    and "ctx `` {k} \<subseteq> set (corder k)"
+    and "distinct (corder k)"
+  shows "Max (view_of corder ctx k) < length (corder k)"
+  using assms
+  by (simp add: view_of_in_range)
+
+
 lemma read_done_kvs_of_s:
   assumes "read_done cl kvt_map sn u'' s s'"
-    and "\<forall>k. Commit_Order_Sound' s k"
-    and "\<forall>k. Commit_Order_Sound' s' k"
+    and "\<forall>k. CO_Distinct s k"
+    and "\<forall>k. Cl_Ctx_Sub_CO s k"
+    and "\<forall>k. Get_Ctx_Sub_CO s k"
+    and "\<forall>k. T0_in_CO s k"
+    and "View_Init s cl"
     and "Rtxn_IdleK_notin_rs s cl"
     and "Rtxn_RegK_in_rs s cl"
   shows "kvs_of_s s' = update_kv (get_txn s cl)
-    (\<lambda>k. case_op_type (map_option fst (kvt_map k)) None)
-    (view_of (commit_order s) (cl_ctx (cls s cl) \<union> get_ctx s kvt_map))
-    (kvs_of_s s)"
+          (\<lambda>k. case_op_type (map_option fst (kvt_map k)) None)
+          (view_of (commit_order s) (cl_ctx (cls s cl) \<union> get_ctx s kvt_map))
+          (kvs_of_s s)"
   using assms
   apply (auto simp add: update_kv_defs update_kv_writes_def update_kv_reads_def)
-  apply (rule ext) apply (auto split: option.split ver_state.split)
-  subgoal apply (auto simp add: Commit_Order_Sound'_def read_done_def kvs_of_s_def
-        split: ver_state.split)
+  apply (rule ext) apply (auto split: option.split)
+  subgoal apply (auto simp add: read_done_def kvs_of_s_def split: ver_state.split)
     by (smt (verit, best) Rtxn_IdleK_notin_rs_def domIff less_antisym txid0.collapse)
-  subgoal apply (auto simp add: Commit_Order_Sound'_def read_done_def Let_def kvs_of_s_def) oops
+  subgoal for k
+    apply (auto simp add: Let_def last_version_def kvs_of_s_def
+        CO_Distinct_def[of s k])
+    apply (subst map_list_update) oops
 
 end
